Structure/TwoStructure.lean
@@ -8,3 +8,41 @@
 
 
 import Structure.Basic
+
+
+
+open Morphisms
+open Functors
+open HasStructure
+open Structure
+
+
+
+-- A 2-structure is simply a structure where equivalences are (1-)structures.
+-- We can reuse `HasIsomorphisms` because it accepts generic equivalences; however we additionally need
+-- the combinations of `trans`/`comp_congrArg` and `symm`/`inv_congrArg` to be functorial.
+
+class HasTwoStructure (α : Sort u) where
+(M       : GeneralizedRelation α Structure)
+[hasIsos : HasIsomorphisms M]
+[comp_congrArg_left_functor  {a b c : α} (f : M a b) :
+   IsIsomorphismFunctor (iso (M b c)) (mapRelation (λ g => hasIsos.trans f g) (iso (M a c)))
+                        (λ eg => hasIsos.comp_congrArg (id_ f) eg)]
+[comp_congrArg_right_functor {a b c : α} (g : M b c) :
+   IsIsomorphismFunctor (iso (M a b)) (mapRelation (λ f => hasIsos.trans f g) (iso (M a c)))
+                        (λ ef => hasIsos.comp_congrArg ef (id_ g))]
+[inv_congrArg_functor        {a b   : α}             :
+   IsIsomorphismFunctor (iso (M a b)) (mapRelation hasIsos.symm (iso (M b a))) hasIsos.inv_congrArg]
+
+namespace HasTwoStructure
+
+variable {α : Sort u} [h : HasTwoStructure α]
+
+instance hasGeneralStructure : HasGeneralStructure α :=
+{ equivType := Structure,
+  M         := h.M,
+  hasIsos   := h.hasIsos }
+
+instance hasIso : HasIsomorphisms h.M := h.hasIsos
+
+end HasTwoStructure
